loader correctness

examples/Rot13.v
@@ -11,59 +11,74 @@ Require Import Determ.
 
 From compcert.common Require Import LanguageInterface Smallstep Globalenvs.
 From compcert.process Require Import Process.
+Require Import Asm.
 Import Memory Values Integers ListNotations.
 Require Import CompCertStrat.
 Close Scope list.
 Close Scope Z_scope.
 
-Definition P : esig := {| op := unit; ar _ := nat |}.
-Inductive F_op : Type := F_read : nat -> F_op | F_write : list byte -> F_op.
+Axiom (Hwin: Archi.win64 = false).
+
+Ltac eprod_crush :=
+  repeat
+    (match goal with
+     | [ H: ?a * ?b |- _ ] => destruct H;cbn [fst snd] in *; subst
+     | [ H: (?a, ?b) = (?c, ?d) |- _ ] => inv H
+     | [ H: (?x * ?y)%rel _ _ |- _] => destruct H; cbn [fst snd] in *; subst
+     | [ H: ?x /\ ?y |- _] => destruct H
+     | [ H: (exists _, _) |- _] => destruct H
+     | [ H: unit |- _] => destruct H
+     end).
+
+Definition P : esig := {| op := Genv.symtbl; ar _ := Integers.int |}.
+Inductive F_op : Type := F_read : Integers.int64 -> F_op | F_write : list byte -> F_op.
 Definition F : esig :=
   {|
     op := F_op;
-    ar m := match m with F_read _ => list byte | F_write _ => nat end;
+    ar m := match m with F_read _ => list byte | F_write _ => Integers.int end;
   |}.
 Definition S : esig := F + F.
 
 Arguments compose_when {E F G}%esig_scope {i j k} p (σ τ)%strat_scope.
 
+Definition emp : Genv.symtbl := Genv.empty_stbl nil.
 Definition Γ_play : @play S P ready :=
-  @oq S P tt ::
-  @pq S P tt (inr (F_write hello_bytes)) ::
-  @oa S P tt (inr (F_write hello_bytes)) 5 ::
-  @pa S P tt 0 :: pnil_ready.
+  @oq S P emp ::
+  @pq S P emp (inr (F_write hello_bytes)) ::
+  @oa S P emp (inr (F_write hello_bytes)) (Int.repr 5) ::
+  @pa S P emp (Int.repr 0) :: pnil_ready.
 Definition Γ : S ->> P := down Γ_play.
 Definition Γ_secret_play : @play S P ready :=
-  @oq S P tt ::
-  @pq S P tt (inr (F_write uryyb_bytes)) ::
-  @oa S P tt (inr (F_write uryyb_bytes)) 5 ::
-  @pa S P tt 0 :: pnil_ready.
+  @oq S P emp ::
+  @pq S P emp (inr (F_write uryyb_bytes)) ::
+  @oa S P emp (inr (F_write uryyb_bytes)) (Int.repr 5) ::
+  @pa S P emp (Int.repr 0) :: pnil_ready.
 Definition Γ_secret : S ->> P := down Γ_secret_play.
 Definition Γ_decode_play : @play S P ready :=
-  @oq S P tt ::
-  @pq S P tt (inl (F_read 100)) ::
-  @oa S P tt (inl (F_read 100)) uryyb_bytes ::
-  @pq S P tt (inr (F_write hello_bytes)) ::
-  @oa S P tt (inr (F_write hello_bytes)) 5 ::
-  @pa S P tt 0 :: pnil_ready.
+  @oq S P emp ::
+  @pq S P emp (inl (F_read (Int64.repr 100))) ::
+  @oa S P emp (inl (F_read (Int64.repr 100))) uryyb_bytes ::
+  @pq S P emp (inr (F_write hello_bytes)) ::
+  @oa S P emp (inr (F_write hello_bytes)) (Int.repr 5) ::
+  @pa S P emp (Int.repr 0) :: pnil_ready.
 Definition Γ_decode : S ->> P := down Γ_decode_play.
 Definition seq_play n1 n2: @play (P + P) P ready :=
-  @oq (P+P) P tt ::
-  @pq (P+P) P tt (inl tt) ::
-  @oa (P+P) P tt (inl tt) n1 ::
-  @pq (P+P) P tt (inr tt) ::
-  @oa (P+P) P tt (inr tt) n2 ::
-  @pa (P+P) P tt n2 :: pnil_ready.
+  @oq (P+P) P emp ::
+  @pq (P+P) P emp (inl emp) ::
+  @oa (P+P) P emp (inl emp) n1 ::
+  @pq (P+P) P emp (inr emp) ::
+  @oa (P+P) P emp (inr emp) n2 ::
+  @pa (P+P) P emp n2 :: pnil_ready.
 Definition seq : P + P ->> P := sup n1, sup n2, down (seq_play n1 n2).
 Inductive fifo_play: list byte -> forall i, @play 0 F i -> Prop :=
 | fifo_nil d : fifo_play d ready pnil_ready
 | fifo_read n d1 d2 d s
-    (Hd: d = app d1 d2) (Hn: n = length d1) (Hs: fifo_play d2 ready s):
+    (Hd: d = app d1 d2) (Hn: Int64.unsigned n = Z.of_nat (length d1)) (Hs: fifo_play d2 ready s):
   fifo_play d ready (@oq 0 F (F_read n) :: @pa 0 F (F_read n) d1 :: s)
-| fifo_read_all n d s (Hn: n > length d) (Hs: fifo_play nil ready s):
+| fifo_read_all n d s (Hn: (Int64.unsigned n > Z.of_nat (length d))%Z) (Hs: fifo_play nil ready s):
   fifo_play d ready (@oq 0 F (F_read n) :: @pa 0 F (F_read n) d :: s)
 | fifo_write n d1 d2 d s
-    (Hd: d2 = app d d1) (Hn: n = length d1) (Hs: fifo_play d2 ready s):
+    (Hd: d2 = app d d1) (Hn: Int.unsigned n = Z.of_nat (length d1)) (Hs: fifo_play d2 ready s):
   fifo_play d ready (@oq 0 F (F_write d1) :: @pa 0 F (F_write d1) n :: s).
 Program Definition fifo : 0 ->> F :=
   {|
@@ -98,7 +113,7 @@ Proof.
   2: { eauto using Downset.closed. } clear Hp. unfold pipe.
   unfold compose at 1. cbn - [compose].
   eexists _, _. repeat apply conj.
-  { exists 0, 0. reflexivity. }
+  { exists (Int.repr 0), (Int.repr 0). reflexivity. }
   2: { unfold Γ_play, seq_play.
        apply comp_oq. apply comp_lq. apply comp_ra.
        repeat constructor. }
@@ -153,8 +168,10 @@ Proof.
   eexists _, _. repeat apply conj.
   cbn. apply fdel_question_l. apply fdel_answer_l. apply fdel_question_r. apply fdel_answer_r. apply fdel_ready.
   cbn. eapply fifo_write with (d1 := uryyb_bytes).
-  rewrite app_nil_l. reflexivity. cbn. reflexivity.
-  eapply fifo_read_all with (n := 100). cbn. lia. apply fifo_nil.
+  rewrite app_nil_l. reflexivity. cbn.
+  instantiate (1 := (Int.repr 5)). reflexivity.
+  eapply fifo_read_all with (n := (Int64.repr 100)). cbn.
+  rewrite Int64.unsigned_repr. lia. cbn. lia. apply fifo_nil.
 
   repeat constructor.
   repeat constructor.
@@ -167,7 +184,7 @@ Proof.
   eexists _, _. repeat apply conj.
   cbn. apply frhor_ready.
   cbn. apply id_has_q with (m := F_write hello_bytes).
-  apply id_has_a with (n := 5). apply id_has_pnil_ready.
+  apply id_has_a with (n := (Int.repr 5)). apply id_has_pnil_ready.
 
   eapply fcomp_oq_r.
   eapply (fcomp_pq_r (E1 := F) (E2 := F)).
@@ -175,3 +192,675 @@ Proof.
   eapply (fcomp_pa_r (E1 := F) (E2 := F)).
   constructor.
 Qed.
+
+Require Import CAsm Load InitMem Maps AST.
+Require Import Conventions Mach Asm.
+
+Context (read_id write_id: ident).
+Section C_LOADER.
+  Import Ctypes Clight.
+  Context (prog: Clight.program).
+  Let sk := AST.erase_program prog.
+
+  Definition entry_c_play (se: Genv.symtbl) q r i : @play li_c P ready :=
+    @oq li_c P se ::
+    @pq li_c P se (se, q)%embed ::
+    @oa li_c P se (se, q)%embed r ::
+    @pa li_c P se i :: pnil_ready.
+  Inductive valid_entry_c: Genv.symtbl -> c_query -> c_reply -> int -> Prop :=
+  | valid_entry_c_intro se b m main f q r i m'
+    (HM: init_mem se sk = Some m)
+    (HB: Genv.find_symbol se main = Some b)
+    (HMAIN: prog_main prog = Some main)
+    (HF: (prog_defmap prog) ! main = Some (Gfun f))
+    (HQ: q = cq (Vptr b Ptrofs.zero) main_sig []%list m)
+    (HR: r = cr (Vint i) m') :
+    valid_entry_c se q r i.
+  Definition entry_c : li_c ->> P :=
+    sup se, sup q, sup r, sup i, sup (_: valid_entry_c se q r i), down (entry_c_play se q r i).
+
+  Definition read_c_play se q n bytes r : @play S li_c ready :=
+    @oq S li_c (se, q)%embed ::
+    @pq S li_c (se, q)%embed (inl (F_read n)) ::
+    @oa S li_c (se, q)%embed (inl (F_read n)) bytes ::
+    @pa S li_c (se, q)%embed r :: pnil_ready.
+  Inductive valid_read_c: Genv.symtbl -> c_query -> Int64.int -> list byte -> c_reply -> Prop :=
+  | valid_read_c_intro se q r vf b ofs n m bytes m'
+    (HVF: Genv.find_funct (Clight.globalenv se prog) vf = Some read)
+    (HREAD: Mem.storebytes m b (Ptrofs.unsigned ofs) (map Byte bytes) = Some m')
+    (HLEN: (Z.of_nat (length bytes) <= Int64.unsigned n)%Z)
+    (HQ: q = cq vf rw_sig [Vint (Int.repr 0); Vptr b ofs; Vlong n]%list m)
+    (HR: r = cr (Vint (Int.repr (Z.of_nat (length bytes)))) m') :
+    valid_read_c se q n bytes r.
+  Definition read_c : S ->> li_c :=
+    sup se, sup q, sup n, sup bytes, sup r, sup (_: valid_read_c se q n bytes r), down (read_c_play se q n bytes r).
+  Definition write_c_play se q bytes n r : @play S li_c ready :=
+    @oq S li_c (se, q)%embed ::
+    @pq S li_c (se, q)%embed (inr (F_write bytes)) ::
+    @oa S li_c (se, q)%embed (inr (F_write bytes)) n ::
+    @pa S li_c (se, q)%embed r :: pnil_ready.
+  Inductive valid_write_c: Genv.symtbl -> c_query -> list byte -> Int.int -> c_reply -> Prop :=
+  | valid_write_c_intro se q r vf b ofs len n m bytes 
+    (HVF: Genv.find_funct (Clight.globalenv se prog) vf = Some write)
+    (HWRITE: Mem.loadbytes m b (Ptrofs.unsigned ofs) len = Some (map Byte bytes))
+    (HQ: q = cq vf rw_sig [Vint (Int.repr 1); Vptr b ofs; Vlong (Int64.repr len)]%list m)
+    (HR: r = cr (Vint n) m) :
+    valid_write_c se q bytes n r.
+  Definition write_c : S ->> li_c :=
+    sup se, sup q, sup bytes, sup n, sup r, sup (_: valid_write_c se q bytes n r), down (write_c_play se q bytes n r).
+  Definition runtime_c : S ->> li_c := join read_c write_c.
+  Definition load_c_prog : S ->> P :=
+    entry_c ⊙ (lts_strat (Clight.semantics1 prog)) ⊙ runtime_c.
+  Definition load_c_sem (L: Smallstep.semantics li_c li_c) : S ->> P :=
+    entry_c ⊙ (lts_strat L) ⊙ runtime_c.
+
+End C_LOADER.
+
+Section ASM_LOADER.
+  Import Asm.
+  Context (prog: Asm.program).
+  Let sk := erase_program prog.
+
+  Definition entry_asm_play (se: Genv.symtbl) q r rv : @play li_asm P ready :=
+    @oq li_asm P se ::
+    @pq li_asm P se (se, q)%embed ::
+    @oa li_asm P se (se, q)%embed r ::
+    @pa li_asm P se rv :: pnil_ready.
+  Inductive valid_entry_asm: Genv.symtbl -> (regset * Mem.mem) -> (regset * Mem.mem) -> int -> Prop :=
+  | valid_entry_asm_intro se rs m rs' m' i vf b f main
+    (HM: init_mem se sk = Some m)
+    (HMAIN: prog_main prog = Some main)
+    (HF: (prog_defmap prog) ! main = Some (Gfun f))
+    (HB: Genv.find_symbol se main = Some b)
+    (HVF: vf = Vptr b Ptrofs.zero)
+    (HRS: rs = (((Pregmap.init Vundef) # PC <- vf) # RSP <- vf) # RA <- Vnullptr)
+    (HRS': rs'#(IR RAX) = Vint i) :
+    valid_entry_asm se (rs, m) (rs', m') i.
+  Definition entry_asm : li_asm ->> P :=
+    sup se, sup q, sup r, sup i, sup (_: valid_entry_asm se q r i), down (entry_asm_play se q r i).
+  Definition read_asm_play se q n bytes r : @play S li_asm ready :=
+    @oq S li_asm (se, q)%embed ::
+    @pq S li_asm (se, q)%embed (inl (F_read n)) ::
+    @oa S li_asm (se, q)%embed (inl (F_read n)) bytes ::
+    @pa S li_asm (se, q)%embed r :: pnil_ready.
+  Inductive valid_read_asm: Genv.symtbl -> (regset * Mem.mem) -> Int64.int -> list byte -> (regset * Mem.mem) -> Prop :=
+  | valid_read_asm_intro se (rs: regset) m n bytes rs' m' b ofs
+      (HVF: Genv.find_funct (Genv.globalenv se prog) rs#PC = Some read_asm)
+      (HDI: rs#RDI = Vint (Int.repr 0))
+      (HSI: rs#RSI = Vptr b ofs)
+      (HDX: rs#RDX = Vlong n)
+      (HN: (Z.of_nat (length bytes) <= Int64.unsigned n)%Z)
+      (HM: Mem.storebytes m b (Ptrofs.unsigned ofs) (map Byte bytes) = Some m')
+      (HAX: rs'#(IR RAX) = Vint (Int.repr (Z.of_nat (length bytes)))) :
+    valid_read_asm se (rs, m) n bytes (rs', m').
+  Definition read_asm : S ->> li_asm :=
+    sup se, sup q, sup n, sup bytes, sup r, sup (_: valid_read_asm se q n bytes r), down (read_asm_play se q n bytes r).
+  Definition write_asm_play se q bytes n r : @play S li_asm ready :=
+    @oq S li_asm (se, q)%embed ::
+    @pq S li_asm (se, q)%embed (inr (F_write bytes)) ::
+    @oa S li_asm (se, q)%embed (inr (F_write bytes)) n ::
+    @pa S li_asm (se, q)%embed r :: pnil_ready.
+  Inductive valid_write_asm: Genv.symtbl -> (regset * Mem.mem) -> list byte -> Int.int -> (regset * Mem.mem) -> Prop :=
+  | valid_write_asm_intro se (rs: regset) m bytes n rs' b ofs r
+      (HVF: Genv.find_funct (Genv.globalenv se prog) rs#PC = Some write_asm)
+      (HDI: rs#RDI = Vint (Int.repr 1))
+      (HSI: rs#RSI = Vptr b ofs)
+      (HDX: rs#RDX = Vlong (Int64.repr n))
+      (HM: Mem.loadbytes m b (Ptrofs.unsigned ofs) n = Some (map Byte bytes))
+      (HAX: rs'#(IR RAX) = Vint r) :
+    valid_write_asm se (rs, m) bytes r (rs', m).
+  Definition write_asm : S ->> li_asm :=
+    sup se, sup q, sup bytes, sup n, sup r, sup (_: valid_write_asm se q bytes n r), down (write_asm_play se q bytes n r).
+  Definition runtime_asm : S ->> li_asm := join read_asm write_asm.
+  Definition load_asm_prog : S ->> P :=
+    entry_asm ⊙ (lts_strat (Asm.semantics prog)) ⊙ runtime_asm.
+  Definition load_asm_sem (L: Smallstep.semantics li_asm li_asm) : S ->> P :=
+    entry_asm ⊙ (lts_strat L) ⊙ runtime_asm.
+
+End ASM_LOADER.
+
+Section LOADER_CORRECT.
+  Import Clight Ctypes.
+  Transparent Archi.ptr64.
+
+  Context p tp (Hp: Compiler.transf_clight_program p = Errors.OK tp).
+  Context
+    (Hromatch: forall se m, init_mem se (AST.erase_program p) = Some m ->
+        ValueAnalysis.romatch_all se (VAInject.bc_of_symtbl se) m).
+
+  Lemma Hsk: erase_program p = erase_program tp.
+  Proof.
+    eapply match_prog_skel; eauto. apply Compiler.transf_clight_program_match. eauto.
+  Qed.
+
+  Lemma entry_correct: rsq CAsm.cc_compcert vid (entry_c p) (entry_asm tp).
+  Proof.
+    intros x (se & q & r & i & H & Hx). inv H. cbn in Hx. rewrite Hx. clear Hx.
+    assert (Hmain: (prog_defmap (erase_program p)) ! main = Some (Gfun tt)).
+    { rewrite erase_program_defmap. unfold option_map. setoid_rewrite HF. reflexivity. }
+    assert (exists tf, (prog_defmap tp) ! main = Some (Gfun tf)) as (tf & Htf).
+    { rewrite Hsk in Hmain. rewrite erase_program_defmap in Hmain.
+      unfold option_map in Hmain.
+      destruct (prog_defmap tp) ! main as [[tf|]|] eqn: Htf; inv Hmain.
+      exists tf. split; eauto. }
+    assert (Htpmain: AST.prog_main tp = Some main).
+    { replace (AST.prog_main tp) with (AST.prog_main (erase_program tp)) by reflexivity.
+      rewrite <- Hsk. apply HMAIN. }
+    unfold entry_c_play. apply rsp_oq. {
+      cbn. eexists se, (_, m), ((Pregmap.init Vundef)#RAX <- (Vint i), m'), i.
+      eexists. econstructor; eauto.
+      - rewrite <- Hsk. eauto.
+      - constructor. }
+    intros q Hq. cbn in Hq. subst q.
+    set (rs :=  (((Pregmap.init Vundef) # PC <- (Vptr b Ptrofs.zero)) # RSP <- (Vptr b Ptrofs.zero)) # RA <- Vnullptr).
+    eapply rsp_pq with (m2 := (se, Datatypes.pair rs m)%embed).
+
+    assert (exists w, LanguageInterface.match_query cc_compcert w
+      {| cq_vf := Vptr b Ptrofs.zero; cq_sg := main_sig; cq_args := []; cq_mem := m |} (rs, m) /\ match_senv cc_compcert w se se).
+    {
+      eexists. split.
+      - unfold cc_compcert.
+        (* cklr *)
+        cbn. instantiate (1 := (se, existT _ 0%nat _, _)).
+        exists (cq (Vptr b Ptrofs.zero) main_sig [] m). split.
+        { reflexivity. }
+        (* inv wt_c *)
+        instantiate (1 := (se, (se, main_sig), _)).
+        exists (cq (Vptr b Ptrofs.zero) main_sig [] m). split.
+        { repeat constructor. }
+        (* lessdef_c *)
+        instantiate (1 := (se, tt, _)).
+        exists (cq (Vptr b Ptrofs.zero) main_sig [] m). split.
+        { repeat constructor. }
+        (* cc_c_asm *)
+        instantiate (1 := (se, caw main_sig
+                    (((Pregmap.init Vundef) # PC
+                      <- (Vptr b Ptrofs.zero)# RSP
+                      <- (Vptr b Ptrofs.zero))# RA
+                     <- Vnullptr) m, _)).
+        eexists ((((Pregmap.init Vundef) # PC
+                   <- (Vptr b Ptrofs.zero)) # RSP
+                  <- (Vptr b Ptrofs.zero)) # RA
+                 <- Vnullptr, m). split.
+        { econstructor; cbn; try constructor; eauto.
+          - destruct Archi.win64; cbn; try easy.
+          - repeat constructor. red. unfold size_arguments.
+            cbn. destruct Archi.win64; reflexivity.
+          - erewrite init_mem_nextblock; eauto.
+            exploit @Genv.genv_symb_range; eauto.
+          - easy.
+          - easy. }
+        (* cc_asm vainj *)
+        instantiate (1 := (se, Inject.injw (Mem.flat_inj (Mem.nextblock m)) (Mem.nextblock m) (Mem.nextblock m))).
+        repeat apply conj; cbn; eauto; try easy.
+        + intros.
+          assert (Val.inject (Mem.flat_inj (Mem.nextblock m)) (Vptr b Ptrofs.zero) (Vptr b Ptrofs.zero)).
+          { eapply Val.inject_ptr. unfold Mem.flat_inj.
+             destruct plt. reflexivity.
+             exfalso. apply n. erewrite init_mem_nextblock; eauto.
+             eapply Genv.genv_symb_range; eauto.
+             reflexivity. }
+          destruct r; eauto; cbn; try constructor; eauto.
+          destruct i0; eauto; cbn.
+        + constructor; cbn.
+          * erewrite init_mem_nextblock; eauto. reflexivity.
+          * eapply Hromatch. eauto.
+          * constructor. eapply initmem_inject; eauto.
+      - cbn. repeat apply conj; eauto. constructor. eauto.
+        constructor; cbn; erewrite init_mem_nextblock; eauto; try easy.
+        apply match_stbls_flat_inj.
+    }
+
+    destruct H as (w & Hq & Hse).  econstructor; eauto.
+    eapply rsp_oa. {
+      cbn. eexists se, (_, m), ((Pregmap.init Vundef)#RAX <- (Vint i), m'), i.
+      eexists. econstructor; eauto.
+      - rewrite <- Hsk. eauto.
+      - repeat constructor. }
+    intros [rs1 m1] Hr. eapply rcp_forbid_mr in Hr; eauto.
+    3: {
+      unfold cc_compcert.
+      (* cklr *)
+      cbn. instantiate (1 := (se, existT _ 0%nat _, _)).
+      exists (cq (Vptr b Ptrofs.zero) main_sig [] m). split.
+      { reflexivity. }
+      (* inv wt_c *)
+      instantiate (1 := (se, (se, main_sig), _)).
+      exists (cq (Vptr b Ptrofs.zero) main_sig [] m). split.
+      { repeat constructor. }
+      (* lessdef_c *)
+      instantiate (1 := (se, tt, _)).
+      exists (cq (Vptr b Ptrofs.zero) main_sig [] m). split.
+      { repeat constructor. }
+      (* cc_c_asm *)
+      instantiate (1 := (se, caw main_sig
+                               (((Pregmap.init Vundef) # PC
+                                 <- (Vptr b Ptrofs.zero)# RSP
+                                 <- (Vptr b Ptrofs.zero))# RA
+                                <- Vnullptr) m, _)).
+      eexists ((((Pregmap.init Vundef) # PC
+                 <- (Vptr b Ptrofs.zero)) # RSP
+                <- (Vptr b Ptrofs.zero)) # RA
+               <- Vnullptr, m). split.
+      { econstructor; cbn; try constructor; eauto.
+        - destruct Archi.win64; cbn; try easy.
+        - repeat constructor. red. unfold size_arguments.
+          cbn. destruct Archi.win64; reflexivity.
+        - erewrite init_mem_nextblock; eauto.
+          exploit @Genv.genv_symb_range; eauto.
+        - easy.
+        - easy. }
+      (* cc_asm vainj *)
+      instantiate (1 := (se, Inject.injw (Mem.flat_inj (Mem.nextblock m)) (Mem.nextblock m) (Mem.nextblock m))).
+      repeat apply conj; cbn; eauto; try easy.
+      + intros.
+        assert (Val.inject (Mem.flat_inj (Mem.nextblock m)) (Vptr b Ptrofs.zero) (Vptr b Ptrofs.zero)).
+        { eapply Val.inject_ptr. unfold Mem.flat_inj.
+          destruct plt. reflexivity.
+          exfalso. apply n. erewrite init_mem_nextblock; eauto.
+          eapply Genv.genv_symb_range; eauto.
+          reflexivity. }
+        destruct r; eauto; cbn; try constructor; eauto.
+        destruct i0; eauto; cbn.
+      + constructor; cbn.
+        * erewrite init_mem_nextblock; eauto. reflexivity.
+        * eapply Hromatch. eauto.
+        * constructor. eapply initmem_inject; eauto.
+    }
+    2: {
+      cbn. repeat apply conj; eauto. constructor. eauto.
+      constructor; cbn; erewrite init_mem_nextblock; eauto; try easy.
+      apply match_stbls_flat_inj.
+    }
+    cbn in Hr. destruct Hr as (r3 & Hr3 & HR). inv Hr3.
+    destruct HR as (r3 & Hr3 & HR). inv Hr3.
+    destruct HR as (r3 & Hr3 & HR). inv Hr3. inv H3.
+    destruct HR as (r3 & Hr3 & HR). inv Hr3. cbn in *.
+    destruct HR as ((? & ?) & ? & Hr). 
+    inv Hr. specialize (H1 RAX). rewrite <- H5 in H1.
+    cbn in H1. inv H1.
+
+    eapply rsp_pa with (r2 := i).
+    { intros Hx. inv Hx. apply H3. apply JMeq_refl. }
+    apply rsp_ready. cbn. eexists _, (rs, _), (rs1, _), _. eexists.
+    { econstructor; eauto.
+      * rewrite <- Hsk. eauto.
+      * subst rs. cbn. rewrite H12. easy. }
+    unfold entry_asm_play. reflexivity.
+    Unshelve. all: cbn; exact tt.
+  Qed.
+
+  Import Compiler CKLR CallconvAlgebra VAInject Inject.
+  Definition inj_state := (block * ptrofs * Mem.mem)%type.
+  Inductive match_inj_state:
+    ccworld (cc_cklrs^{*}) -> world vainj -> cc_ca_world -> inj_state -> inj_state -> Prop := 
+  | match_inj_state_intro wn wi b1 ofs1 m1 b2 ofs2 m2 caw se 
+      (HM: mm_ca wn (se, wi) (caw_m caw) m1 m2) (HP: mp_ca wn wi b1 ofs1 b2 ofs2):
+      match_inj_state wn (se, wi) caw (b1, ofs1, m1) (b2, ofs2, m2).
+  Instance runtime_asm_determ:
+    Deterministic (runtime_asm tp).
+  Admitted.
+
+  Lemma runtime_correct: rsq vid CAsm.cc_compcert (runtime_c p) (runtime_asm tp).
+  Proof.
+    setoid_rewrite cc_conv_expand. apply rsq_sup. apply runtime_asm_determ.
+    { constructor. apply None. }
+    intros [w|].
+    2: { intros s ([|] & Hs).
+         - destruct Hs as (se & q & n & bs & r & H & Hs). rewrite Hs. clear Hs.
+           unfold read_c_play. apply rsp_oq. {
+             exists true. cbn. inv H. eexists se, (((((Pregmap.init Vundef)#PC <- vf)#RDI <- (Vint (Int.repr 0))#RSI <- (Vptr b ofs))#RDX <- (Vlong n)), m), n, bs, ((Pregmap.init Vundef)#RAX <- (Vint (Int.repr (Z.of_nat (Datatypes.length bs)))), m').
+             eexists. 2: constructor.
+             econstructor; cbn; eauto.
+             eapply match_prog_read. 4: eauto.
+             apply Compiler.transf_clight_program_match. eauto.
+             apply Genv.match_stbls_id.
+             apply val_inject_refl. }
+           intros q2 Hq2. xinv Hq2.
+         - destruct Hs as (se & q & bs & n & r & H & Hs). rewrite Hs. clear Hs.
+           unfold write_c_play. apply rsp_oq. {
+             exists false. cbn. inv H. eexists se, (((((Pregmap.init Vundef)#PC <- vf)#RDI <- (Vint (Int.repr 1))#RSI <- (Vptr b ofs))#RDX <- (Vlong (Int64.repr len))), m), bs, n, ((Pregmap.init Vundef)#RAX <- (Vint n), m).
+             eexists. 2: constructor.
+             econstructor; cbn; eauto.
+             eapply match_prog_write. 4: eauto.
+             apply Compiler.transf_clight_program_match. eauto.
+             apply Genv.match_stbls_id.
+             apply val_inject_refl. }
+           intros q2 Hq2. xinv Hq2. }
+    intros s (i & Hs). destruct i; cbn in Hs.
+    Ltac inv_lessdef:=
+      match goal with
+      | [ H: Val.lessdef_list _ _ |- _ ] => inv H
+      | [ H: Val.lessdef _ _ |- _ ] => inv H
+      end.
+    - destruct Hs as (se & q & n & bs & r & H & Hs). rewrite Hs. clear Hs.
+      inv H. unfold read_c_play. apply rsp_oq. {
+        exists true. cbn. eexists se, (((((Pregmap.init Vundef)#PC <- vf)#RDI <- (Vint (Int.repr 0))#RSI <- (Vptr b ofs))#RDX <- (Vlong n)), m), n, bs, ((Pregmap.init Vundef)#RAX <- (Vint (Int.repr (Z.of_nat (Datatypes.length bs)))), m').
+        eexists. 2: constructor.
+        econstructor; cbn; eauto.
+        eapply match_prog_read. 4: eauto.
+        apply Compiler.transf_clight_program_match. eauto.
+        apply Genv.match_stbls_id.
+        apply val_inject_refl.
+      }
+      intros q Hq. cbn in Hq. dependent destruction Hq.
+      eapply rsp_pq with (m2 := inl (F_read n)). reflexivity.
+      eapply rsp_oa. {
+        exists true. cbn. 
+      set (w1 := (nw_of_world w)). set (w2 := (injw_of_world w)). set (w3 := (caw_of_world w)).
+      unfold CAsm.cc_compcert in *. cbn in w, HM |- *.
+      eprod_crush. destruct s7.
+      match goal with
+      | [ H: Invariant.rel_inv _ _ _ |- _ ] => inv H; eprod_crush; subst
+      end.
+      (* cklrs *)
+      eapply (cklrs_match_query_inv (existT _ x2 c0)) in H as
+          (mx & bx & ofsx & vfx & Hqx & Hmx & Hpx & Hvx). subst x0. cbn in *.
+      (* lessdef *)
+      inv H1. repeat inv_lessdef.
+      (* cc_c_asm: need to show args_removed changes nothing *)
+      inv H2. inv HRM. inv H.
+      2: { match goal with
+          | [ H: size_arguments _ > 0 |- _ ] => rewrite rw_sig_size_arguments in H  end.
+           lia. apply Hwin. }
+      (* cc_asm vainj *)
+      destruct m2. destruct H3 as (Hreg & Hpc & Him).
+      (* arguments *)
+      match goal with
+      | [ H: cons _ _ = _ |- _ ] => cbn in H; rewrite Hwin in H; cbn in H; inv H
+      end.
+
+      assert (exists b' ofs', r0#RSI = Vptr b' ofs' /\ Val.inject i (Vptr bx ofsx) (Vptr b' ofs')) as (b' & ofs' & Hofs & Hb').
+      { specialize (Hreg RSI). rewrite <- H2 in Hreg. inv Hreg.
+        eexists _, _. split; eauto. }
+
+      assert (HMS: match_inj_state w1 w2 w3 (b, ofs, m) (b', ofs', m0)).
+      { econstructor.
+        (* mem *)
+        - inv Him. econstructor; eauto. reflexivity.
+          cbn. apply Mem.unchanged_on_refl.
+        (* ptr *)
+        - econstructor; eauto. inv Hb'. constructor; eauto. }
+      inv HMS.
+      exploit ca_storebytes; eauto. intros (mx1 & Hs & Hm).
+      inv Hm.
+
+        eexists _, _, _, _, ((Pregmap.init Vundef)#RAX <- (Vint (Int.repr (Z.of_nat (Datatypes.length bs)))), _).
+        eexists.
+        2: { unfold read_asm_play. repeat constructor. }
+        econstructor; eauto.
+      + cbn in HVF. cbn in HSE.  eprod_crush. inv H8.
+        eapply ca_find_funct_read; eauto.
+        apply Compiler.transf_clight_program_match. eauto.
+        apply H7. apply HVF.
+      + specialize (Hreg RDI). rewrite <- H0 in Hreg. inv Hreg; eauto.
+      + specialize (Hreg RDX). rewrite <- H3 in Hreg. inv Hreg; eauto.
+      }
+      intros r2 H2. cbn in H2. apply not_and_or in H2 as [H2|H2]. easy.
+      assert (bs = r2) as <-.
+      { apply NNPP. intros Hx. apply H2. intros Hy. apply Hx.
+        apply JMeq_eq; eauto. } clear H2.
+
+      set (w1 := (nw_of_world w)). set (w2 := (injw_of_world w)). set (w3 := (caw_of_world w)).
+      unfold CAsm.cc_compcert in *. cbn in w, HM |- *.
+      eprod_crush. destruct s7.
+      match goal with
+      | [ H: Invariant.rel_inv _ _ _ |- _ ] => inv H; eprod_crush; subst
+      end.
+      (* cklrs *)
+      eapply (cklrs_match_query_inv (existT _ x2 c0)) in H as
+          (mx & bx & ofsx & vfx & Hqx & Hmx & Hpx & Hvx). subst x0. cbn in *.
+      (* lessdef *)
+      inv H1. repeat inv_lessdef.
+      (* cc_c_asm: need to show args_removed changes nothing *)
+      inv H2. inv HRM. inv H.
+      2: { match goal with
+          | [ H: size_arguments _ > 0 |- _ ] => rewrite rw_sig_size_arguments in H  end.
+           lia. apply Hwin. }
+      (* cc_asm vainj *)
+      destruct m2. destruct H3 as (Hreg & Hpc & Him).
+      (* arguments *)
+      match goal with
+      | [ H: cons _ _ = _ |- _ ] => cbn in H; rewrite Hwin in H; cbn in H; inv H
+      end.
+
+      assert (exists b' ofs', r0#RSI = Vptr b' ofs' /\ Val.inject i (Vptr bx ofsx) (Vptr b' ofs')) as (b' & ofs' & Hofs & Hb').
+      { specialize (Hreg RSI). rewrite <- H2 in Hreg. inv Hreg.
+        eexists _, _. split; eauto. }
+
+      assert (HMS: match_inj_state w1 w2 w3 (b, ofs, m) (b', ofs', m0)).
+      { econstructor.
+        (* mem *)
+        - inv Him. econstructor; eauto. reflexivity.
+          cbn. apply Mem.unchanged_on_refl.
+        (* ptr *)
+        - econstructor; eauto. inv Hb'. constructor; eauto. }
+      inv HMS.
+      exploit ca_storebytes; eauto. intros (mx1 & Hs & Hm).
+      inv Hm.
+      set (v := (Vint (Int.repr (Z.of_nat (length bs))))).
+      eapply rsp_pa with (r2 := ((r0#RAX <- v)#PC <- (r0#RA), mx1)).
+      {
+        intros HR. cbn in HR. dependent destruction HR. apply HN0. clear HM0 HN0.
+
+        (* m --store--> m'
+           |            |
+           |          mm_cklr
+           |            |
+         mm_ca          m2
+           |            |
+           |           inj
+           |            |
+          m0 --store--> mx1
+         *)
+
+        eexists (cr v m2). split.
+        { eapply cklrs_match_reply_intro; eauto. }
+        eexists (cr v m2). split.
+        (* need sig *)
+        { constructor. easy. }
+        eexists (cr v m2). split.
+        { constructor. constructor. }
+        exists ((r#RAX <- v)#PC <- (r#RA), m2). split.
+        { cbn in Hreg |- *.
+          (* destruct w3; cbn in HSG, HRS |- *. *)
+          (* subst caw_sg.  *)
+          constructor; eauto.
+          - intros r1. destruct r1; cbn; eauto. easy.
+          - apply Mem.unchanged_on_refl.
+          - rewrite rw_sig_size_arguments.
+            replace (loc_init_args 0 (r RSP))
+              with (fun (_: block) (_: Z) => False); eauto.
+            repeat (apply Axioms.functional_extensionality; intros).
+            apply PropExtensionality.propositional_extensionality.
+            split; try easy. intros HX. inv HX. lia.
+            apply Hwin.
+          - rewrite rw_sig_size_arguments.
+            intros * HX. inv HX. lia.
+            apply Hwin. }
+        { exists (s0, wj). split. split; eauto. split.
+          - intros. cbn in Hreg. apply (mi_acc inj) in HJ.
+            destruct r1; cbn; eauto. 
+            destruct i0; cbn; eauto.
+            subst v. eauto.
+          - constructor; eauto. }
+      }
+
+      apply rsp_ready. exists true.
+      eexists _, (r0, m0), _, _, ((r0#RAX <- v)#PC <- (r0#RA), mx1).
+      eexists.
+      { econstructor; eauto.
+      + cbn in HVF. cbn in HSE.  eprod_crush. inv r1.
+        eapply ca_find_funct_read; eauto.
+        apply Compiler.transf_clight_program_match. eauto.
+        apply m1. apply HVF.
+      + specialize (Hreg RDI). rewrite <- H0 in Hreg. inv Hreg; eauto.
+      + specialize (Hreg RDX). rewrite <- H3 in Hreg. inv Hreg; eauto. }
+      cbn. reflexivity.
+    - destruct Hs as (se & q & bs & n & r & H & Hs). rewrite Hs. clear Hs.
+      inv H. unfold write_c_play. apply rsp_oq. {
+        exists false. cbn. eexists se, (((((Pregmap.init Vundef)#PC <- vf)#RDI <- (Vint (Int.repr 1))#RSI <- (Vptr b ofs))#RDX <- (Vlong (Int64.repr len))), m), bs, n, ((Pregmap.init Vundef)#RAX <- (Vint n), m).
+        eexists. 2: constructor.
+        econstructor; cbn; eauto.
+        eapply match_prog_write. 4: eauto.
+        apply Compiler.transf_clight_program_match. eauto.
+        apply Genv.match_stbls_id.
+        apply val_inject_refl.
+      }
+      intros q Hq. cbn in Hq. dependent destruction Hq.
+      eapply rsp_pq with (m2 := inr (F_write bs)). reflexivity.
+      eapply rsp_oa. {
+        exists false. cbn.
+
+      set (w1 := (nw_of_world w)). set (w2 := (injw_of_world w)). set (w3 := (caw_of_world w)).
+      destruct m2 as [rs mt].
+      unfold CAsm.cc_compcert in *. cbn in w, HM |- *.
+      eprod_crush. destruct s7.
+      match goal with
+      | [ H: Invariant.rel_inv _ _ _ |- _ ] => inv H; eprod_crush; subst
+      end.
+      eapply (cklrs_match_query_inv (existT _ x2 c0)) in H as
+          (mx & bx & ofsx & vfx & Hqx & Hmx & Hpx & Hvx). subst x0. cbn in *.
+      (* lessdef *)
+      inv H1. repeat inv_lessdef.
+      (* cc_c_asm: need to show args_removed changes nothing *)
+      inv H2. inv HRM. inv H.
+      2: { match goal with
+        | [ H: size_arguments _ > 0 |- _ ] =>
+            rewrite rw_sig_size_arguments in H; try lia  end. apply Hwin. }
+      (* cc_asm vainj *)
+      destruct H3 as (Hreg & Hpc & Him).
+      (* arguments *)
+      match goal with
+      | [ H: cons _ _ = _ |- _ ] => cbn in H; rewrite Hwin in H; cbn in H; inv H
+      end.
+      assert (exists b' ofs', rs#RSI = Vptr b' ofs' /\ Val.inject i (Vptr bx ofsx) (Vptr b' ofs')) as (b' & ofs' & Hofs & Hb').
+      { specialize (Hreg RSI). rewrite <- H2 in Hreg. inv Hreg.
+        eexists _, _. split; eauto. }
+      assert (HCA: mm_ca w1 w2 (caw_m w3) m mt).
+      { inv Him. econstructor; eauto. reflexivity.
+        apply Mem.unchanged_on_refl. }
+
+        eexists _, _, _, _, ((Pregmap.init Vundef)#RAX <- (Vint n), _).
+        exists. 2: { repeat constructor. }
+         econstructor; cbn; eauto.
+        + cbn in HVF. cbn in HSE.  eprod_crush. inv H8.
+          eapply ca_find_funct_write; eauto.
+          apply Compiler.transf_clight_program_match. eauto.
+          apply H7. apply HVF.
+        + specialize (Hreg RDI). rewrite <- H0 in Hreg. inv Hreg; eauto.
+        + specialize (Hreg RDX). rewrite <- H3 in Hreg. inv Hreg; eauto.
+        + inv Him. eapply ca_loadbytes; eauto.
+          econstructor; eauto. inv Hb'. constructor; eauto.
+      }
+      intros r2 H2. cbn in H2. apply not_and_or in H2 as [H2|H2]. easy.
+      assert (n = r2) as <-.
+      { apply NNPP. intros Hx. apply H2. intros Hy. apply Hx.
+        apply JMeq_eq; eauto. } clear H2.
+      set (w1 := (nw_of_world w)). set (w2 := (injw_of_world w)). set (w3 := (caw_of_world w)).
+      destruct m2 as [rs mt].
+      unfold CAsm.cc_compcert in *. cbn in w, HM |- *.
+      eprod_crush. destruct s7.
+      match goal with
+      | [ H: Invariant.rel_inv _ _ _ |- _ ] => inv H; eprod_crush; subst
+      end.
+      eapply (cklrs_match_query_inv (existT _ x2 c0)) in H as
+          (mx & bx & ofsx & vfx & Hqx & Hmx & Hpx & Hvx). subst x0. cbn in *.
+      (* lessdef *)
+      inv H1. repeat inv_lessdef.
+      (* cc_c_asm: need to show args_removed changes nothing *)
+      inv H2. inv HRM. inv H.
+      2: { match goal with
+        | [ H: size_arguments _ > 0 |- _ ] =>
+            rewrite rw_sig_size_arguments in H; try lia  end. apply Hwin. }
+      (* cc_asm vainj *)
+      destruct H3 as (Hreg & Hpc & Him).
+      (* arguments *)
+      match goal with
+      | [ H: cons _ _ = _ |- _ ] => cbn in H; rewrite Hwin in H; cbn in H; inv H
+      end.
+      assert (exists b' ofs', rs#RSI = Vptr b' ofs' /\ Val.inject i (Vptr bx ofsx) (Vptr b' ofs')) as (b' & ofs' & Hofs & Hb').
+      { specialize (Hreg RSI). rewrite <- H2 in Hreg. inv Hreg.
+        eexists _, _. split; eauto. }
+      
+      set (v := (Vint n)).
+      eapply rsp_pa with (r2 := ((rs#RAX <- v)#PC <- (rs#RA), mt)).
+      {
+        intros HR. cbn in HR. dependent destruction HR. apply HN. clear HM HN.
+        eexists (cr v mx). split.
+        { eapply cklrs_match_reply_intro; eauto. }
+        eexists (cr v mx). split.
+        (* need sig *)
+        { constructor. easy. }
+        eexists (cr v mx). split.
+        { constructor. constructor. }
+        exists ((r#RAX <- v)#PC <- (r#RA), mx). split.
+        { cbn in Hreg |- *. constructor; eauto.
+          - intros r1. destruct r1; cbn; eauto. easy.
+          - apply Mem.unchanged_on_refl.
+          - apply Mem.unchanged_on_refl.
+          - rewrite rw_sig_size_arguments.
+            intros * HX. inv HX. lia. apply Hwin. }
+        { exists (s0, i). split. reflexivity. split; eauto.
+          intros. cbn in Hreg. destruct r0; cbn; eauto. destruct i0; cbn; eauto.
+          subst v. eauto. }
+      }
+
+      assert (HCA: mm_ca w1 w2 (caw_m w3) m mt).
+      { inv Him. econstructor; eauto. reflexivity.
+        apply Mem.unchanged_on_refl. }
+
+      apply rsp_ready. exists false.
+      eexists _, (rs, mt), _, _, ((rs#RAX <- v)#PC <- (rs#RA), mt).
+      eexists.
+      { econstructor; eauto.
+        + cbn in HVF. cbn in HSE.  eprod_crush. inv r0.
+          eapply ca_find_funct_write; eauto.
+          apply Compiler.transf_clight_program_match. eauto.
+          apply m0. apply HVF.
+        + specialize (Hreg RDI). rewrite <- H0 in Hreg. inv Hreg; eauto.
+        + specialize (Hreg RDX). rewrite <- H3 in Hreg. inv Hreg; eauto.
+        + inv Him. eapply ca_loadbytes; eauto.
+          econstructor; eauto. inv Hb'. constructor; eauto.
+        + cbn. reflexivity. }
+      cbn. reflexivity.
+  Qed.
+
+  Lemma load_sem_correct L_c L_asm:
+    determinate L_asm ->
+    forward_simulation CAsm.cc_compcert CAsm.cc_compcert L_c L_asm ->
+    load_c_sem p L_c [= load_asm_sem tp L_asm.
+  Proof.
+    intros HD HL. eapply rsq_id_conv with (p := rs_ready).
+    eapply rsq_comp_when. constructor. apply entry_correct.
+    eapply rsq_comp_when. constructor. 2: apply runtime_correct.
+    apply fsim_rsq; eauto.
+  Qed.
+
+  (* Lemma load_prog_correct : *)
+  (*   load_c_prog p [= load_asm_prog tp. *)
+  (* Admitted. *)
+End LOADER_CORRECT.
+
+Require process.Secret.
+
+Section SECRET.
+  Hypothesis (Hwin: Archi.win64 = false).
+
+  Definition rot13_c : Clight.program. Admitted.
+  Context rot13_asm (Hrot13: Compiler.transf_clight_program rot13_c = Errors.OK rot13_asm).
+
+  Context (secret_sk: AST.program unit unit).
+  Definition Σ_secret : Smallstep.semantics li_c li_c. Admitted.
+  Lemma ϕ_secret : Γ_secret [= load_c secret_sk Σ_secret. Admitted.
+
+
+  Definition L_secret := Secret.secret_spec.
+  Context compose_secret (HX: SmallstepLinking.compose L_secret (Clight.semantics2 rot13_c) = Some compose_secret).
+  Lemma π_secret : forward_simulation 1%cc 1%cc Σ_secret compose_secret. Admitted.
+
+  Context link_asm (HL: Linking.link rot13_asm Secret.secret_asm_program = Some link_asm).
+  Lemma π_secret_cc : forward_simulation cc_compcert cc_compcert Σ_secret (Asm.semantics link_asm).
+  Admitted.
+
+End SECRET.
